upgraded Lean

src/util/data/array.lean
@@ -1,7 +1,9 @@
 
 import data.list
-
+import data.list.basic
+import data.array.lemmas
 import util.data.fin
+import util.data.list
 import util.data.order
 
 universe variables u₀ u₁ u₂
@@ -15,41 +17,38 @@ def push_aux {n : ℕ} (x : α) (ar : fin n → α) : fin (succ n) → α
   | ⟨0,_⟩ := x
   | ⟨succ i,P⟩ := ar ⟨i,lt_of_succ_lt_succ P⟩
 
-def push {n : ℕ} (x : α) : array α n → array α (succ n)
+def push {n : ℕ} (x : α) : array n α → array (succ n) α
   | ⟨ ar ⟩ := ⟨ push_aux x ar ⟩
 
-def pop {n : ℕ} : array α (succ n) → array α n
+def pop {n : ℕ} : array (succ n) α → array n α
   | ⟨ ar ⟩ := ⟨ ar ∘ fin.succ ⟩
 
-def head {n : ℕ} : array α (succ n) → α
+def head {n : ℕ} : array (succ n) α → α
   | ⟨ ar ⟩ := ar 0
 
-lemma push_head_pop {n : ℕ} (xs : array α (succ n))
+lemma push_head_pop {n : ℕ} (xs : array (succ n) α)
 : push (head xs) (pop xs) = xs := sorry
 
+open d_array -- (rev_iterate_aux rev_iterate)
 lemma rev_iterate_push {n : ℕ}
-  (x : α) (xs : array α n)
+  (x : α) (xs : array n α)
   (i : β)
   (f : fin (succ n) → α → β → β)
 : rev_iterate (push x xs) i f = f 0 x (rev_iterate xs i (f ∘ fin.succ)) :=
 begin
   revert x xs,
   induction n with n IH ; intros x xs,
-  { cases xs with xs,
-    unfold push push_aux rev_iterate rev_iterate_aux,
-    simp,
-    unfold read data push_aux,
-    rw fin.zero_def', refl },
+  { cases xs with xs, refl, },
   { rw [← push_head_pop xs,IH],
     unfold function.comp,
-    rw push_head_pop xs,
+    rw [push_head_pop xs],
     admit }
 end
 
-def maximum_aux {n : ℕ} (a : array ℕ n) (i : ℕ) (H : i ≤ n) : ℕ :=
-array.iterate_aux a (λ _, max) i H 0
+def maximum_aux {n : ℕ} (a : array n ℕ) (i : ℕ) (H : i ≤ n) : ℕ :=
+d_array.iterate_aux a (λ _, max) i H 0
 
-lemma le_maximum_aux {n : ℕ} (a : array ℕ n) (k : ℕ) (Hk : k ≤ n)
+lemma le_maximum_aux {n : ℕ} (a : array n ℕ) (k : ℕ) (Hk : k ≤ n)
   (i  : fin n)
   (Hi : i.val < k)
 : a.read i ≤ maximum_aux a k Hk :=
@@ -61,25 +60,25 @@ begin
     simp, admit },
 end
 
-def maximum {n : ℕ} (a : array ℕ n) : ℕ :=
+def maximum {n : ℕ} (a : array n ℕ) : ℕ :=
 maximum_aux a n (by refl)
 
-lemma le_maximum {n : ℕ} (a : array ℕ n) (i : fin n)
+lemma le_maximum {n : ℕ} (a : array n ℕ) (i : fin n)
 : a.read i ≤ maximum a :=
 begin
   apply le_maximum_aux,
   apply i.is_lt
 end
 
-lemma rev_list_eq_nil (ar : array α 0)
+lemma rev_list_eq_nil (ar : array 0 α)
 : ar.rev_list = [] :=
 by refl
 
-lemma to_list_eq_nil (ar : array α 0)
+lemma to_list_eq_nil (ar : array 0 α)
 : ar.to_list = [] :=
 by refl
 
-lemma iterate_aux_pop {n : ℕ} (ar : array α (succ n))
+lemma iterate_aux_pop {n : ℕ} (ar : array (succ n) α)
   (f : fin (succ n) → α → β → β) (x : β)
   {k : ℕ}
   (Hk : k ≤ n)
@@ -90,13 +89,13 @@ begin
   case zero
     { refl },
   case succ k
-    { rw array.iterate_aux.equations._eqn_2 (pop ar), simp,
+    { rw d_array.iterate_aux.equations._eqn_2 (pop ar), simp,
       rw ← ih_1, unfold iterate_aux, simp,
       apply congr_fun,
       cases ar, refl }
 end
 
-lemma rev_list_eq_cons_aux {n k : ℕ} (ar : array α n) (xs : list α)
+lemma rev_list_eq_cons_aux {n k : ℕ} (ar : array n α) (xs : list α)
   (H : k ≤ n)
 : iterate_aux ar (λ _, list.cons) k H xs =
       iterate_aux ar (λ _, list.cons) k H [] ++ xs :=
@@ -106,14 +105,14 @@ begin
   { unfold iterate_aux, simp [ih_1], },
 end
 
-lemma rev_list_eq_cons {n : ℕ} (ar : array α (succ n))
+lemma rev_list_eq_cons {n : ℕ} (ar : array (succ n) α)
 : ar.rev_list = ar.pop.rev_list ++ [ar.read 0] :=
 begin
-  unfold rev_list foldl iterate,
+  unfold rev_list foldl iterate d_array.iterate,
   rw [iterate_aux_pop _ _ _ (le_refl n),rev_list_eq_cons_aux],
 end
 
-lemma iterate_aux_pop_back {n : ℕ} (ar : array α (succ n))
+lemma iterate_aux_pop_back {n : ℕ} (ar : array (succ n) α)
   (f : fin (succ n) → α → β → β) (x : β)
   (k : ℕ)
   (Hk : k ≤ n)
@@ -128,10 +127,10 @@ begin
       apply ih_1 },
 end
 
-lemma rev_list_eq_append {n : ℕ} (ar : array α (succ n))
+lemma rev_list_eq_append {n : ℕ} (ar : array (succ n) α)
 : ar.rev_list = ar.read fin.max :: ar.pop_back.rev_list :=
 begin
-  unfold rev_list foldl iterate iterate_aux,
+  unfold rev_list foldl iterate d_array.iterate iterate_aux,
   simp,
   apply congr_arg,
   apply iterate_aux_pop_back,
@@ -143,40 +142,39 @@ lemma fin.sum_zero
   [has_add α] [has_zero α]
   (f : fin 0 → α)
 : fin.sum 0 f = 0 :=
-begin
-  unfold fin.sum fin.foldl,
-  rw [array.foldl_eq,array.rev_list_eq_nil],
-  refl,
-end
-
+rfl
+open array
 lemma fin.sum_succ {n : ℕ}
   [add_comm_monoid α]
   (f : fin (succ n) → α)
 : fin.sum (succ n) f = fin.sum n (f ∘ fin.succ) + f 0 :=
 begin
   unfold fin.sum fin.foldl,
-  simp [array.foldl_eq,array.rev_list_eq_cons],
-  unfold array.read array.data array.pop,
+  repeat { rw [← rev_list_foldr] },
+  simp [d_array.foldl,array.rev_list_eq_cons,d_array.iterate,d_array.iterate_aux
+       ,read,d_array.read,d_array.data,array.pop],
   symmetry,
   rw list.foldr_hom (has_add.add (f 0)), simp,
   intros, simp
 end
 
+@[simp]
+lemma array_widen_eq_pop_back {n : ℕ} (f : fin (succ n) → α)
+: d_array.mk (f ∘ widen) = array.pop_back ⟨f⟩ :=
+begin
+  simp [array.pop_back],
+  apply array.ext,
+  intro,
+  cases i, refl,
+end
+
+open list
 lemma fin.sum_succ' {n : ℕ}
   [add_comm_monoid α]
   (f : fin (succ n) → α)
 : fin.sum (succ n) f = fin.sum n (f ∘ widen) + f fin.max :=
 begin
   unfold fin.sum fin.foldl,
-  rw [array.foldl_eq,array.foldl_eq,array.rev_list_eq_append],
-  unfold list.foldr array.read array.data,
-  rw [add_comm],
-  apply congr_fun,
-  apply congr_arg,
-  apply congr_arg,
-  apply congr_arg,
-  unfold array.pop_back,
-  apply congr_arg,
-  apply funext, intro, cases x with i Hi,
-  refl,
+  rw [← to_list_foldl,← to_list_foldl],
+  simp [foldl_eq_foldr',rev_list_eq_append,foldr,flip,read,d_array.read],
 end
